feat: progress
praise be to mario

Std/Data/HashMap/Lemmas.lean
@@ -21,71 +21,37 @@ theorem List.eraseP_eq_filter_of_unique (l : List α) (p : α → Bool)
     | false => simp [eraseP_cons, filter, hP, ih]
 
 @[simp]
-theorem Array.foldl_zero {as : Array α} {init : β} {f : β → α → β}
-    : as.foldl f init (stop := 0) = init := by
-  sorry
-
-@[simp]
-theorem Array.foldl_succ {as : Array α} {init : β} {f : β → α → β} (i : Fin as.size)
-    : as.foldl f init (stop := i + 1) = f (as.foldl f init (stop := i)) as[i] := by
-  sorry
-
-theorem Array.foldlM_zero [Monad m] [LawfulMonad m]
-    {as : Array α} {init : β} {f : β → α → m β} {start : Nat}
-    : as.foldlM f init start 0 = pure init := by
-  unfold foldlM foldlM.loop
-  simp [Nat.not_lt_zero]
-
-theorem Array.foldlM_succ [Monad m] [LawfulMonad m]
-    {as : Array α} {init : β} {f : β → α → m β} {start : Nat} (i : Fin as.size) : start ≤ i.val
-    → (as.foldlM f init start (i.val + 1)) = as.foldlM f init start i >>= (f · as[i]) := by
-  intro hStartLe
-  have hISuccLe : i.val + 1 ≤ as.size := Nat.succ_le_of_lt i.isLt
-  have hILe : i.val ≤ as.size := Nat.le_of_lt i.isLt
-  simp only [foldlM, hISuccLe, hILe, dite_true]
-  conv => lhs; unfold foldlM.loop
-  simp only [Nat.lt_succ_of_le hStartLe, dite_true]
-  split
-  case h_1 h =>
-    exfalso
-    exact Nat.le_trans (Nat.sub_eq_zero_iff_le.mp h) hStartLe
-      |> Nat.lt_of_succ_le
-      |> Nat.not_lt_of_le (Nat.le_refl _)
-  case h_2 h =>
-    -- This is kinda tricky, since foldlM recurses on start rather than stop. Rethink..
-    sorry
+theorem List.foldl_cons_fn (l₁ l₂ : List α) :
+    l₁.foldl (init := l₂) (fun acc x => x :: acc) = l₁.reverse ++ l₂ := by
+  induction l₁ generalizing l₂ <;> simp [*]
 
 namespace Std.HashMap
 open List
 
 variable [BEq α] [Hashable α] [LawfulHashable α] [PartialEquivBEq α]
 
-/-- It is a bit easier to reason about `fold (append)` than `fold (fold)`,
-so we transfer most proofs about `toList` from this auxiliary function. -/
-def toList' (m : HashMap α β) : List (α × β) :=
+/-- It is a bit easier to reason about `foldl (append)` than `foldl (foldl)`, so we use this
+(less efficient) variant of `toList` as the mathematical model. -/
+def toListModel (m : HashMap α β) : List (α × β) :=
   m.val.buckets.val.foldl (init := []) (fun acc bkt => acc ++ bkt.toList)
 
--- TODO: naming
-theorem foldl_induction₂ {as : Array α} (motive : Nat → β → β → Prop) {init₁ init₂ : β}
-    (h0 : motive 0 init₁ init₂) {f g : β → α → β}
-    (hf : ∀ i : Fin as.size, ∀ acc₁ acc₂,
-      motive i.1 acc₁ acc₂ → motive (i.1 + 1) (f acc₁ as[i]) (g acc₂ as[i]))
-    : motive as.size (as.foldl f init₁) (as.foldl g init₂) := by
-  apply Array.foldl_induction
-    (motive := fun i (acc : β) => motive i acc (as.foldl g init₂ (stop := i)))
-    (h0 := Array.foldl_zero ▸ h0)
-    (hf := fun _ _ hPrev => by rw [Array.foldl_succ]; exact hf _ _ _ hPrev)
-
-theorem toList_perm_toList' (m : HashMap α β) : m.toList' ~ m.toList := by
-  unfold toList toList' HashMap.fold HashMap.Imp.fold
-  apply foldl_induction₂ (fun _ l₁ l₂ => l₁ ~ l₂) (h0 := List.Perm.nil)
-  intro acc₁ acc₂ l hAcc
-  sorry
+theorem toList_eq_reverse_toListModel (m : HashMap α β) : m.toList = m.toListModel.reverse := by
+  simp only [toList, toListModel, fold, Imp.fold, Array.foldl_eq_foldl_data, AssocList.foldl_eq,
+    List.foldl_cons_fn]
+  suffices ∀ (l₁ : List (AssocList α β)) (l₂ : List (α × β)),
+      l₁.foldl (init := l₂.reverse) (fun d b => b.toList.reverse ++ d) =
+      (l₁.foldl (init := l₂) fun acc bkt => acc ++ bkt.toList).reverse by
+    apply this (l₂ := [])
+  intro l₁
+  induction l₁ with
+  | nil => intro; rfl
+  | cons a as ih =>
+    intro l₂
+    simp only [List.foldl, ← List.reverse_append, ih]
 
 /-- The map does not store duplicate (`beq`) keys. -/
-theorem Pairwise_bne_toList (m : HashMap α β) : m.toList.Pairwise (·.1 != ·.1) := by
-  apply List.Perm.pairwise_iff (bne_symm _ _) (toList_perm_toList' m) |>.mp
-  unfold toList'
+theorem Pairwise_bne_toListModel (m : HashMap α β) : m.toListModel.Pairwise (·.1 != ·.1) := by
+  unfold toListModel
   refine Array.foldl_induction
     (motive := fun i (acc : List (α × β)) =>
       -- The acc has the desired property
@@ -123,53 +89,62 @@ theorem Pairwise_bne_toList (m : HashMap α β) : m.toList.Pairwise (·.1 != ·.
           exact .trans hHashP.symm hHashR
         exact Nat.ne_of_lt hGt this
 
-theorem toList_eraseP_eq_toList_filter (m : HashMap α β)
-    : m.toList.eraseP (·.1 == a) = m.toList.filter (·.1 != a) := by
+theorem toListModel_eraseP_eq_toListModel_filter (m : HashMap α β)
+    : m.toListModel.eraseP (·.1 == a) = m.toListModel.filter (·.1 != a) := by
   apply List.eraseP_eq_filter_of_unique
-  apply List.Pairwise.imp ?_ (Pairwise_bne_toList _)
+  apply List.Pairwise.imp ?_ (Pairwise_bne_toListModel _)
   intro (a₁, _) (a₂, _) hA₁Bne hA₁Beq
   rw [Bool.not_eq_true_iff_ne_true]
   intro hA₂Beq
   exact Bool.not_bne_of_beq (PartialEquivBEq.trans hA₁Beq (PartialEquivBEq.symm hA₂Beq)) hA₁Bne
 
-theorem toList_insert_perm_cons_eraseP (m : HashMap α β) (a : α) (b : β)
-    : (m.insert a b).toList ~ (a, b) :: m.toList.eraseP (·.1 == a) :=
+theorem toListModel_insert_perm_cons_eraseP (m : HashMap α β) (a : α) (b : β)
+    : (m.insert a b).toListModel ~ (a, b) :: m.toListModel.eraseP (·.1 == a) :=
   sorry
 
-theorem toList_insert (m : HashMap α β) (a : α) (b : β)
-    : (m.insert a b).toList ~ (a, b) :: m.toList.filter (·.1 != a) :=
-  toList_eraseP_eq_toList_filter m ▸ toList_insert_perm_cons_eraseP m a b
+theorem toListModel_insert (m : HashMap α β) (a : α) (b : β)
+    : (m.insert a b).toListModel ~ (a, b) :: m.toListModel.filter (·.1 != a) :=
+  toListModel_eraseP_eq_toListModel_filter m ▸ toListModel_insert_perm_cons_eraseP m a b
 
-theorem toList_erase_perm_eraseP (m : HashMap α β) (a : α)
-    : (m.erase a).toList ~ m.toList.eraseP (·.1 == a) :=
+theorem toListModel_erase_perm_eraseP (m : HashMap α β) (a : α)
+    : (m.erase a).toListModel ~ m.toListModel.eraseP (·.1 == a) :=
   sorry
 
-theorem toList_erase (m : HashMap α β) (a : α)
-    : (m.erase a).toList ~ m.toList.filter (·.1 != a) :=
-  toList_eraseP_eq_toList_filter m ▸ toList_erase_perm_eraseP m a
+theorem toListModel_erase (m : HashMap α β) (a : α)
+    : (m.erase a).toListModel ~ m.toListModel.filter (·.1 != a) :=
+  toListModel_eraseP_eq_toListModel_filter m ▸ toListModel_erase_perm_eraseP m a
 
-theorem find?_of_toList_contains (m : HashMap α β) (a : α) (b : β)
-    : (∃ a', a == a' ∧ (a', b) ∈ m.toList) ↔ m.find? a = some b :=
+theorem findEntry?_eq (m : HashMap α β) (a : α)
+    : m.findEntry? a = m.toListModel.find? (·.1 == a) := by
+  unfold findEntry? Imp.findEntry?
+  conv => simp_match; simp_match
   sorry
 
-theorem find?_of_toList_not_contains (m : HashMap α β) (a : α)
-    : (∀ a' (b : β), a == a' → (a', b) ∉ m.toList) ↔ m.find? a = none := by
+theorem find?_of_toListModel_contains (m : HashMap α β) (a : α) (b : β)
+    : (∃ a', a == a' ∧ (a', b) ∈ m.toListModel) ↔ m.find? a = some b := by
+  unfold HashMap.toListModel HashMap.find? Imp.find?
+  -- have H : (∃ a', a == a' ∧ (a', b) ∈ m.toListModel)
+  --     ↔ (∃ a', ∃ bkt, (i : Fin m.val.buckets.val.size) → bkt = m.val.buckets.val[i] → (a',b) ∈ bkt) := sorry
+  sorry
+
+theorem find?_of_toListModel_not_contains (m : HashMap α β) (a : α)
+    : (∀ a' (b : β), a == a' → (a', b) ∉ m.toListModel) ↔ m.find? a = none := by
   apply Iff.intro
   . rw [← Option.not_isSome_iff_eq_none]
     intro h hSome
     let ⟨b, hB⟩ := Option.isSome_iff_exists.mp hSome
-    let ⟨a', hA, hMem⟩ := find?_of_toList_contains m a b |>.mpr hB
+    let ⟨a', hA, hMem⟩ := find?_of_toListModel_contains m a b |>.mpr hB
     exact h a' b hA hMem
   . intro h a' b hA hMem
     refine Option.ne_none_iff_exists.mpr ?_ h
-    exact ⟨b, find?_of_toList_contains m a b |>.mp ⟨a', hA, hMem⟩ |>.symm⟩
+    exact ⟨b, find?_of_toListModel_contains m a b |>.mp ⟨a', hA, hMem⟩ |>.symm⟩
 
 theorem find?_insert (m : HashMap α β) (a a' b)
     : a' == a → (m.insert a b).find? a' = some b := by
   intro hEq
-  apply (find?_of_toList_contains _ _ _).mp
+  apply (find?_of_toListModel_contains _ _ _).mp
   refine ⟨a, hEq, ?_⟩
-  rw [List.Perm.mem_iff (toList_insert m a b)]
+  rw [List.Perm.mem_iff (toListModel_insert m a b)]
   apply List.mem_cons_self
 
 theorem find?_insert_of_ne (m : HashMap α β) (a a' : α) (b : β)
@@ -178,7 +153,7 @@ theorem find?_insert_of_ne (m : HashMap α β) (a a' : α) (b : β)
   apply Option.ext
   intro b'
   show find? (insert m a b) a' = some b' ↔ find? m a' = some b'
-  simp only [← find?_of_toList_contains, List.Perm.mem_iff (toList_insert m a b), List.mem_cons,
+  simp only [← find?_of_toListModel_contains, List.Perm.mem_iff (toListModel_insert m a b), List.mem_cons,
     List.mem_filter, Prod.mk.injEq]
   apply Iff.intro
   . intro ⟨a'', hA', h⟩
@@ -197,9 +172,9 @@ theorem find?_insert_of_ne (m : HashMap α β) (a a' : α) (b : β)
 theorem find?_erase (m : HashMap α β) (a a')
     : a == a' → (m.erase a).find? a' = none := by
   intro hEq
-  apply (find?_of_toList_not_contains _ _).mp
+  apply (find?_of_toListModel_not_contains _ _).mp
   intro a₂ b hA₂ hMem
-  rw [List.Perm.mem_iff (toList_erase m a)] at hMem
+  rw [List.Perm.mem_iff (toListModel_erase m a)] at hMem
   refine Bool.not_bne_of_beq (PartialEquivBEq.symm <| PartialEquivBEq.trans hEq hA₂) ?_
   exact List.mem_filter.mp hMem |>.right
 
